SL/Assertions.thy
@@ -1,5 +1,170 @@
 theory Assertions
-  imports "../Algebra/Quantale"
+  imports "../Algebra/BBI" Heap
 begin
+
+no_notation 
+  times (infixl "*" 70) and
+  bot ("\<bottom>")
+
+type_synonym 'a pred = "('a \<times> heap) set"
+
+definition emp :: "'a pred" where
+  "emp \<equiv> {(s, h). h = Map.empty}"
+
+definition sep :: "'a pred \<Rightarrow> 'a pred \<Rightarrow> 'a pred" (infixl "*" 80) where
+  "p * q \<equiv> {(s, h1 ++ h2) | s h1 h2. h1 \<bottom> h2 \<and> (s, h1) \<in> p \<and> (s, h2) \<in> q}" 
+
+lemma sep_assoc: "p * (q * r) = (p * q) * r"
+  apply (auto simp: sep_def)
+  using Heap.pmult_def_eq apply blast
+  using Heap.pmult_ab1 Heap.pmult_ab2 Heap.pmult_ab_assoc by blast
+
+lemma sep_comm: "p * q = q * p"
+  apply (auto simp: sep_def)
+  using Heap.pmult_comm Heap.pmult_comm_def apply blast
+  using Heap.pmult_comm Heap.pmult_comm_def by blast
+
+section {* Algebraic structure *}
+
+interpretation bbi!: bbi Inf Sup inf less_eq less sup bot top minus uminus sep emp
+  apply default
+  apply (simp_all add: sep_assoc)
+  apply (simp add: sep_comm)
+  apply (auto simp: sep_def emp_def)
+done
+
+abbreviation wand :: "'a pred \<Rightarrow> 'a pred \<Rightarrow> 'a pred" (infixl "-*" 75) where
+  "p -* q \<equiv> bbi.sep_impl p q"
+
+abbreviation (input) 
+  constants :: "'b \<Rightarrow> ('a \<Rightarrow> 'b)" ("#_") where
+  "#x \<equiv> \<lambda>_. x"
+
+abbreviation (input) 
+  pred_ex :: "('b \<Rightarrow> 'a set) \<Rightarrow> 'a set" (binder "EXS " 10) where
+  "EXS x. P x \<equiv> {s. \<exists>x. s \<in> P x}"
+
+abbreviation (input) 
+  pred_all :: "('b \<Rightarrow> 'a set) \<Rightarrow> 'a set" (binder "ALLS " 10) where
+  "ALLS x. P x \<equiv> {s. \<forall>x. s \<in> P x}"
+
+abbreviation (input) 
+  pred_eq :: "('a \<Rightarrow> 'b) \<Rightarrow> ('a \<Rightarrow> 'b) \<Rightarrow> 'a pred" (infix "\<Midarrow>" 50) where
+  "e \<Midarrow> e' \<equiv> {(s, h). e s = e' s}"
+
+no_notation residual_r (infixr "\<rightarrow>" 60)
+abbreviation (input) 
+  pred_impl :: "'a pred \<Rightarrow> 'a pred \<Rightarrow> 'a pred" (infix "\<rightarrow>" 60) where
+  "p \<rightarrow> q \<equiv> (-p) \<squnion> q"
+
+lemma sexI: "P x \<le> (EXS x. P x)"
+  by auto
+
+section {* Variables and Expressions *}
+
+type_synonym ('v, 's) exp = "'s \<Rightarrow> 'v"
+type_synonym 'a nat_exp = "'a \<Rightarrow> nat"
+
+text {* The left value of a variable is an update function. *}
+type_synonym ('v, 's) lval = "('v \<Rightarrow> 'v) \<Rightarrow> 's \<Rightarrow> 's"
+
+text {* The right value of a variable is a retrieve function. *}
+type_synonym ('v, 's) rval = "'s \<Rightarrow> 'v"
+
+text {* A variable is then a pair of left and right values, satisfying some properties. *}
+type_synonym ('v, 's) var = "('v, 's) lval \<times> ('v, 's) rval"
+
+abbreviation subst :: "('s \<Rightarrow> 'v) \<Rightarrow> ('v, 's) lval \<Rightarrow> ('v, 's) rval \<Rightarrow> 's \<Rightarrow> 'v" where
+  "subst e u_upd v \<equiv> \<lambda>s. e (u_upd (\<lambda>_. v s) s)"
+
+abbreviation free :: "('v, 's) lval \<Rightarrow> ('s \<Rightarrow> 'v) \<Rightarrow> bool" where
+  "free u_upd e \<equiv> \<forall>s t. e (u_upd (\<lambda>_. t) s) = e s"
+
+abbreviation vars1 :: "('v, 's) lval \<Rightarrow> ('v, 's) rval \<Rightarrow> bool" where
+  "vars1 u_upd u \<equiv> \<forall>s t. u (u_upd (\<lambda>_. t) s) = t"
+
+abbreviation vars2 :: "('v, 's) lval \<Rightarrow> ('v, 's) rval \<Rightarrow> ('v, 's) rval \<Rightarrow> bool" where
+  "vars2 u_upd u v \<equiv> \<forall>s. u (u_upd (\<lambda>_. v s) s) = v s"
+
+abbreviation vars3 :: "('v, 's) lval \<Rightarrow> ('v, 's) rval \<Rightarrow> bool" where
+  "vars3 u_upd v \<equiv> \<forall>s t. v (u_upd (\<lambda>_. t s) s) = v s"
+
+abbreviation subst_pred :: "('s \<times> 'h) set \<Rightarrow> ('v, 's) lval \<Rightarrow> ('v, 's) rval \<Rightarrow> ('s \<times> 'h) set" where
+  "subst_pred P u t \<equiv> Collect (\<lambda>(s, h). (u (\<lambda>_. t s) s, h) \<in> P)"
+
+abbreviation free_pred :: "('v, 's) lval \<Rightarrow> 's pred \<Rightarrow> bool" where
+  "free_pred v R \<equiv> \<forall>t. R = subst_pred R v t"
+
+section {* Predicates over the Heaplet Model*}
+
+definition singleton :: "'a nat_exp \<Rightarrow> 'a nat_exp \<Rightarrow> 'a pred" ("_ \<mapsto> _" [50, 50] 60) where
+  "e \<mapsto> e' \<equiv> {(s, h). h = [e s \<mapsto> e' s]}"
+
+definition any_singleton :: "'a nat_exp \<Rightarrow> 'a pred" ("_ \<mapsto> -" [50] 60) where
+  "e \<mapsto> - \<equiv> EXS e'. e \<mapsto> e'"
+
+definition points_to :: "'a nat_exp \<Rightarrow> 'a nat_exp \<Rightarrow> 'a pred" ("_ \<hookrightarrow> _" [50, 50] 60) where
+  "e \<hookrightarrow> e' \<equiv> (e \<mapsto> e') * \<top>"
+
+definition any_points_to :: "'a nat_exp \<Rightarrow> 'a pred" ("_ \<hookrightarrow> -" [50] 60) where
+  "e \<hookrightarrow> - \<equiv> (e \<mapsto> -) * \<top>"
+
+definition doublet :: "'a nat_exp \<Rightarrow> 'a nat_exp \<Rightarrow> 'a nat_exp \<Rightarrow> 'a pred" ("_ \<mapsto> _, _" [50, 50, 50] 60) where
+  "e \<mapsto> e1, e2 \<equiv> (e \<mapsto> e1) * ((\<lambda>s. plus (e s) 1) \<mapsto> e2)"
+
+lemma wand_eq: "{(s, h). \<forall>h'. h \<bottom> h' \<and> (s, h') \<in> P \<longrightarrow> (s, h ++ h') \<in> Q} \<le> P -* Q"
+  apply (rule bbi.sep_implI1)
+  apply (clarsimp simp: sep_def)
+done
+
+lemma reynolds1: "(a \<mapsto> a') \<sqinter> (b \<mapsto> b') = (a \<mapsto> a') \<sqinter> (a \<Midarrow> b) \<sqinter> (a' \<Midarrow> b')"
+  apply (auto simp: singleton_def)
+  apply (metis fun_upd_apply option.distinct(1))
+  by (metis fun_upd_apply option.sel)
+
+lemma reynolds2: "(a \<hookrightarrow> a') * (b \<hookrightarrow> b') \<le> -(a \<Midarrow> b)"
+  by (auto simp: points_to_def singleton_def sep_def ortho_def)
+
+lemma alls_exs_eq: "(ALLS x. - P x) = - (EXS x. P x)"
+  by auto
+
+lemma reynolds3_helper: "\<forall>s h. - Q h \<longrightarrow> P (s, h) \<Longrightarrow> - {s. P s} \<subseteq> {(s, h). Q h}"
+  by auto
+
+lemma reynolds3: "emp = (ALLS x. -(x \<hookrightarrow> -))"
+  apply (subst alls_exs_eq)
+  apply (rule antisym)
+  apply (simp add: emp_def)
+  prefer 2
+  apply (subst emp_def)
+  apply (rule reynolds3_helper)
+  apply (auto simp: any_points_to_def any_singleton_def singleton_def sep_def ortho_def)
+  apply (subgoal_tac "\<exists>n. n \<in> dom h")
+  prefer 2
+  apply force
+  apply auto
+  apply (rule_tac x="\<lambda>x. n" in exI)
+  apply (rule_tac x="[n \<mapsto> y]" in exI)
+  apply (rule_tac x="h(n := None)" in exI)
+  apply (auto intro: heap_split)
+  by (metis fun_upd_same map_add_None)
+
+
+lemma reynolds4: "(e \<mapsto> e') * ((e \<mapsto> e') -* p) \<le> (e \<hookrightarrow> e') \<sqinter> p"
+  apply (subst points_to_def)
+  apply (rule bbi.sep_impl_to_meet)
+done
+
+lemma reynolds5_helper: "R * {(s, h). \<forall>h'. h \<bottom> h' \<and> (s, h') \<in> P \<longrightarrow> (s, h ++ h') \<in> Q} \<le> R * (P -* Q)"
+  using bbi.Sup.qisol wand_eq by blast
+
+lemma reynolds5: "(e \<hookrightarrow> e') \<sqinter> p \<le> (e \<mapsto> e') * ((e \<mapsto> e') -* p)"
+  apply (rule order_trans)
+  prefer 2
+  apply (rule reynolds5_helper)
+  apply (auto simp: points_to_def singleton_def sep_def ortho_def)
+  apply (erule_tac x=h2 in allE)
+  apply auto
+  by (simp add: domIff map_add_upd_left)
 
 end
