SL/Heap.thy
@@ -1,0 +1,27 @@
+theory Heap
+  imports Main "../Algebra/PartialMonoid"
+begin
+
+section {* Heaplet Model *}
+
+type_synonym heap = "nat \<Rightarrow> nat option"
+
+definition ortho :: "heap \<Rightarrow> heap \<Rightarrow> bool" (infix "\<bottom>" 55)
+  where "h1 \<bottom> h2 \<equiv> dom h1 \<inter> dom h2 = {}"
+
+lemma theI: "h x = Some y \<Longrightarrow> the (h x) = y"
+  by simp
+
+lemma heap_divider: "h1 \<bottom> h2 \<Longrightarrow> h1 x = Some y \<Longrightarrow> (h1 ++ h2) x = Some y"
+  by (auto simp: ortho_def map_add_def split: option.splits)
+
+lemma heap_add_comm: "h1 \<bottom> h2 \<Longrightarrow> h1 ++ h2 = h2 ++ h1"
+  by (auto simp: ortho_def intro: map_add_comm)
+
+interpretation partial_comm_monoid map_add ortho Map.empty
+  by default (auto simp: ortho_def intro: map_add_comm)
+
+lemma heap_split: "h x = Some y \<Longrightarrow> h = [x \<mapsto> y] ++ h(x := None)"
+  by (metis (mono_tags, lifting) domIff empty_map_add fun_upd_same fun_upd_triv fun_upd_upd map_add_upd_left)
+
+end
