SL/LinkedList.thy
@@ -1,0 +1,141 @@
+theory LinkedList
+  imports StoreHeapModel
+begin
+
+(* Single Linked List *)
+
+abbreviation (input) is_nil :: "'a nat_exp \<Rightarrow> 'a pred" ("_ \<Midarrow> nil") where
+  "i \<Midarrow> nil \<equiv> {(s, h). i s \<notin> dom h}"
+
+primrec llist :: "nat list \<Rightarrow> 'a nat_exp \<Rightarrow> 'a nat_exp \<Rightarrow> 'a pred" where
+  "llist [] i j = emp \<sqinter> (i \<Midarrow> j)"
+| "llist (x#xs) i k = (EXS j. (i \<mapsto> #x, j) * llist xs j k)"
+
+lemma singleton_list [simp]: "(llist [x] i j) = (i \<mapsto> #x, j)"
+  by (auto simp: sep_def doublet_def singleton_def emp_def)
+
+lemma llist_exs: "(EXS j. (emp \<sqinter> (i \<Midarrow> j)) * llist ys j k) = llist ys i k"
+  apply (auto simp: sep_def doublet_def singleton_def emp_def)
+  apply (induct ys)
+  apply (auto simp: doublet_def singleton_def sep_def)
+done
+
+lemma llist_merge: "(llist (xs@ys) i k) = (EXS j. (llist xs i j) * (llist ys j k))"
+  apply (induct xs arbitrary: i)
+  apply (simp add: llist_exs)
+  apply (auto simp: sep_def doublet_def singleton_def emp_def ortho_def
+  sorry
+
+lemma llist_rev: "(llist (xs@[x]) i k) = (EXS j. (llist xs i j) * (j \<mapsto> #x, k))"
+  by (simp add: llist_merge singleton_list del: llist.simps)
+
+lemma "llist xs i j \<le> (i \<Midarrow> nil) \<rightarrow> ((#xs \<Midarrow> #[]) \<sqinter> (i \<Midarrow> nil))"
+  apply (induct xs)
+  apply clarsimp
+  apply (auto simp: sep_def doublet_def singleton_def emp_def ortho_def)
+done
+
+lemma "llist xs i j \<le> (i \<Midarrow> j) \<squnion> - (#xs \<Midarrow> #[])"
+  apply (induct xs)
+  apply clarsimp
+  apply (auto simp: sep_def doublet_def singleton_def emp_def ortho_def)
+done
+
+no_notation sup (infixl "+" 65)
+
+lemma exs1: "(EXS j. (i \<mapsto> a, j) * P j) = (i \<mapsto> a) * (EXS j. ((\<lambda>s. i s + 1) \<mapsto> j) * P j)"
+  apply (auto simp: sep_def doublet_def singleton_def emp_def ortho_def)
+  apply (erule_tac x="[Suc (i s) \<mapsto> x s] ++ h2" in allE)
+  apply auto
+done
+
+lemma tt1: "subst_pred (P * Q) i_update j = (subst_pred P i_update j) * (subst_pred Q i_update j)"
+  by (auto simp: sep_def)
+
+lemma tt2: "subst_pred (EXS k. (P k)) i_update j = (EXS k. (subst_pred (P k) i_update j))"
+  by (auto simp: sep_def)
+
+lemma tt3: "subst_pred (EXS k. (P k) * (Q k)) i_update j = (EXS k. (subst_pred (P k) i_update j) * (subst_pred (Q k) i_update j))"
+  by (auto simp: sep_def)
+
+record test =
+  i :: nat
+  j :: nat
+  k :: nat
+
+lemma tt4: "\<forall>a. x a = subst x i_update j a \<Longrightarrow> subst_pred (i \<mapsto> x) i_update j = j \<mapsto> x"
+  by (auto simp: singleton_def)
+
+lemma tt5: "\<forall>a. x a = subst x i_update j a \<Longrightarrow> subst_pred (i \<mapsto> (\<lambda>_. a), x) i_update j = j \<mapsto> (\<lambda>_. a), x"
+  apply (subst doublet_def)+
+  apply (subst tt1)
+  apply (subst tt4)
+  apply simp
+  apply (subgoal_tac "subst_pred ((\<lambda>s. i s + 1) \<mapsto> x) i_update j = ((\<lambda>s. j s + 1) \<mapsto> x)")
+  apply simp
+  apply (auto simp: singleton_def)
+done
+
+lemma "subst_pred (llist xs i k) i_update j = llist xs j k"
+  apply (induct xs)
+  apply (clarsimp simp add: emp_def)
+  apply force
+
+  apply (subst llist.simps)+
+  apply (subst tt2)
+  apply (subst tt1)
+  apply (subst tt)
+sorry
+
+apply (subst doublet_def)+
+
+
+  apply (auto simp: sep_def doublet_def singleton_def emp_def ortho_def)
+  apply (erule_tac x="subst x i_update j" in allE)
+  apply (erule_tac x=h2 in allE)
+  apply auto
+lemma "ht (llist (Cons x xs) i k)
+    (
+      lookup j_update (\<lambda>s. (i s) + 1);
+      dispose i;
+      dispose (\<lambda>s. i s + 1);
+      assign i_update j
+    )
+    (llist xs i k)"
+    apply (rule hl_seq | rule mptran)+
+prefer 4
+  apply (rule sl)
+  apply (rule order_refl)
+prefer 3
+  apply (rule sl)
+
+
+    apply (rule hl_seq [where r = "llist xs j k"])
+    apply (rule mptran)+
+    apply (rule hl_seq [where r = "((\<lambda>s. i s + 1) \<mapsto> j) * (llist xs j k)"])
+    apply (rule mptran)+
+    apply (rule hl_seq [where r = "(i \<mapsto> #x) * ((\<lambda>s. i s + 1) \<mapsto> j) * (llist xs j k)"])
+    apply (rule mptran)+
+    apply (rule hl_pre [where P' = "(i \<mapsto> #x) * (EXS j. ((\<lambda>s. i s + 1) \<mapsto> j) * (llist xs j k))"])
+
+    apply (simp add: exs1)
+    
+    apply (subst sep_comm)
+    apply (subst sep_comm) back back
+    apply (subst sep_comm) back back back
+    apply (subst sep_assoc)
+    apply (rule sl_frame)
+    apply (rule lptran)
+    apply (simp add: doublet_def singleton_def)
+
+    apply (rule hl_pre)
+prefer 2
+    apply (rule sl_lookup)
+    apply (clarsimp simp: sep_def doublet_def singleton_def emp_def ortho_def)
+    apply (erule_tac x=x in allE)
+    apply (erule_tac x=h2 in allE)
+    apply clarsimp
+    
+    
+    
+end
