SL/StoreHeapModel.thy
@@ -1,0 +1,204 @@
+theory StoreHeapModel
+  imports PredTrans
+begin
+
+type_synonym 'a stran = "'a \<times> heap \<Rightarrow> ('a \<times> heap) option"
+
+definition valid_mem :: "'a option \<Rightarrow> 'a set \<Rightarrow> bool" (infixl "in" 100) where
+  "x in Q \<equiv> case x of None \<Rightarrow> False | Some y \<Rightarrow> y \<in> Q"
+
+definition basic :: "'a stran \<Rightarrow> 'a ptran" ("\<langle>_\<rangle>") where
+  "basic f Q \<equiv> {(s, h). f (s, h) in Q}"
+
+definition assign :: "('v, 's) lval \<Rightarrow> ('s \<Rightarrow>'v) \<Rightarrow> 's ptran" where
+  "assign u_upd t \<equiv> \<langle>\<lambda>(s, h). Some (u_upd (\<lambda>_. t s) s, h)\<rangle>"
+
+definition lookup :: "(nat, 's) lval \<Rightarrow> 's nat_exp \<Rightarrow> 's ptran" where
+  "lookup u_upd t \<equiv> \<langle>\<lambda>(s, h). if t s \<in> dom h
+                              then Some (u_upd (\<lambda>_. the (h (t s))) s, h)
+                              else None\<rangle>"
+
+definition mutation :: "'s nat_exp \<Rightarrow> 's nat_exp \<Rightarrow> 's ptran" where
+  "mutation e t \<equiv> \<langle>\<lambda>(s, h). if e s \<in> dom h
+                            then Some (s, h(e s \<mapsto> t s))
+                            else None\<rangle>"
+(*
+definition cons :: "(nat, 's) lval \<Rightarrow> 's nat_exp \<Rightarrow> 's ptran" where
+  "cons u_upd t \<equiv> \<langle>\<lambda>(s, h). let N = (SOME n. \<forall>x \<in> dom h. n > x) in
+                    Some (u_upd (\<lambda>_. N) s, h(N \<mapsto> t s))\<rangle>"
+*)
+
+definition cons :: "(nat, 's) lval \<Rightarrow> 's nat_exp \<Rightarrow> 's ptran" where
+  "cons u_upd t \<equiv> \<langle>\<lambda>(s, h). let N = (SOME n. n \<notin> dom h) in
+                    Some (u_upd (\<lambda>_. N) s, h ++ [N \<mapsto> t s])\<rangle>"
+
+definition dispose :: "'s nat_exp \<Rightarrow> 's ptran" where
+  "dispose e \<equiv> \<langle>\<lambda>(s, h). if e s \<in> dom h 
+                         then Some (s, h(e s := None)) 
+                         else None\<rangle>"
+
+(* Monotonic *)
+
+lemma mono_basic [mptran]: "mono (basic f)"
+  apply (auto simp: mono_def basic_def valid_mem_def)
+  apply (case_tac "f(a, b)")
+  apply force+
+done
+
+lemma mono_assign [mptran]: "mono (assign u t)"
+  by (auto simp: assign_def intro: mptran)
+
+lemma mono_lookup [mptran]: "mono (lookup u t)"
+  by (auto simp: lookup_def intro: mptran)
+
+lemma mono_mutation [mptran]: "mono (mutation e t)"
+  by (auto simp: mutation_def intro: mptran)
+
+lemma mono_cons [mptran]: "mono (cons u t)"
+  by (auto simp: cons_def intro: mptran)
+
+lemma mono_dispose [mptran]: "mono (dispose e)"
+  by (auto simp: dispose_def intro: mptran)
+
+(* Locality *)
+
+definition basic_local :: "'a stran \<Rightarrow> 'a pred \<Rightarrow> bool" where
+  "basic_local f R \<equiv> \<forall>s h1 h2 Q. h1 \<bottom> h2 \<and> f (s, h1) in Q \<and> (s, h2) \<in> R \<longrightarrow> f(s, h1 ++ h2) in (Q * R)"
+
+lemma local_eq: "local (basic f) R \<longleftrightarrow> basic_local f R"
+  by (force simp: local_def basic_local_def basic_def sep_def)
+
+lemma local_assign: "free_pred v R \<Longrightarrow> local (assign v t) R"
+  by (force simp: local_eq basic_local_def assign_def basic_def sep_def valid_mem_def)
+
+lemma local_lookup [lptran]: "free_pred u R \<Longrightarrow> local (lookup u t) R"
+  apply (auto simp: local_eq basic_local_def lookup_def basic_def sep_def valid_mem_def)
+  apply (rule_tac x=h1 in exI)
+  apply (rule_tac x=h2 in exI)
+  apply (subgoal_tac "the ((h1 ++ h2) (t s)) = y")
+  apply force
+  by (simp add: heap_divider)
+
+lemma local_mutation [lptran]: "local (mutation e t) R"
+  apply (auto simp: local_eq basic_local_def mutation_def basic_def sep_def valid_mem_def)
+  apply (rule_tac x="h1(e s \<mapsto> t s)" in exI)
+  apply (rule_tac x=h2 in exI)
+  apply auto
+  apply (metis (no_types, lifting) dom_fun_upd fun_upd_triv map_add_comm map_add_upd option.distinct(1) ortho_def)
+  apply (auto simp: ortho_def)
+done
+
+lemma "Q n \<Longrightarrow> P (SOME n. Q n) \<Longrightarrow> P n"
+nitpick oops
+
+lemma local_cons [lptran]: "free_pred v R \<Longrightarrow> local (cons u t) R"
+apply (simp add: cons_def local_eq basic_local_def)
+apply auto
+apply (rule_tac someI2_ex)
+defer
+apply (erule conjE)
+apply (subst (asm) someI_ex) 
+oops
+
+
+
+lemma local_dispose [lptran]: "local (dispose e) R"
+  apply (simp add: dispose_def local_def ortho_def sep_def basic_def valid_mem_def)
+  apply auto
+  apply (erule_tac x="h1(e s := None)" in allE)
+  apply auto 
+  apply (erule_tac x="h2" in allE)
+  apply auto
+  apply (auto simp: map_add_def)
+  apply (erule notE)
+  apply (rule ext)
+  apply auto
+  apply (metis disjoint_iff_not_equal domI domIff fun_upd_apply option.case_eq_if)
+  by (metis fun_upd_apply)
+
+
+(* Separation Logic *)
+
+lemma hl_basic [sl]: "P \<subseteq> {s. f s in Q} \<Longrightarrow> ht P (basic f) Q"
+  by (auto simp: ht_def basic_def seq_def)
+
+lemma hl_assign [sl]: "P \<subseteq> subst_pred Q z_upd t \<Longrightarrow> ht P (assign z_upd t) Q"
+  by (auto simp: assign_def valid_mem_def intro!: sl)
+
+lemma sl_mut_local [sl]: "ht (e \<mapsto> -) (mutation e e') (e \<mapsto> e')"
+  by (auto simp: mutation_def valid_mem_def any_singleton_def singleton_def intro!: sl)
+
+lemma sl_mut_global [sl]: "ht ((e \<mapsto> -) * r) (mutation e e') ((e \<mapsto> e') * r)"
+  by (auto intro: sl lptran)
+
+lemma sl_mut [sl]: "ht ((e \<mapsto> -) * ((e \<mapsto> e') -* r)) (mutation e e') r"
+  apply (rule hl_post[where Q'="(e \<mapsto> e') * ((e \<mapsto> e') -* r)"])
+  by (auto simp: Assertions.bbi.sep_impl_annil1 intro!: sl_mut_global mptran)
+
+lemma sl_dipose_local [sl]: "ht (e \<mapsto> -) (dispose e) (emp)"
+  by (auto simp: dispose_def singleton_def valid_mem_def any_singleton_def emp_def intro!: sl)
+
+lemma sl_dispose [sl]: "ht ((e \<mapsto> -) * r) (dispose e) r"
+  by (subst bbi.mult_1[symmetric], (rule sl | rule lptran)+)
+
+lemma sl_alloc_local [sl]: "free u_upd e \<Longrightarrow> vars1 u_upd u \<Longrightarrow> ht emp (cons u_upd e) (u \<mapsto> e)"
+  apply (auto simp: cons_def emp_def valid_mem_def singleton_def intro!: sl)
+  apply (case_tac "let N = SOME n. True in Some (u_upd (\<lambda>_. N) a, [N \<mapsto> e a])")
+  apply (metis option.distinct(1))
+  apply clarsimp
+  apply (simp add: Let_unfold)
+  apply auto
+done
+
+lemma sl_alloc_global [sl]: "free u_upd e \<Longrightarrow> vars1 u_upd u \<Longrightarrow> ht r (cons u_upd e) ((u \<mapsto> e) * r)"
+  oops
+
+lemma sl_alloc  [sl]: "free u_upd e \<Longrightarrow> free_pred u_upd r \<Longrightarrow> ht (ALLS v. (v \<mapsto> e) -* r) (cons u_upd e) r"
+  oops
+
+lemma sl_lookup_local [sl]: "vars2 v_upd v v' \<Longrightarrow> vars3 v_upd v' \<Longrightarrow> free v_upd e \<Longrightarrow> 
+    ht (e \<mapsto> v') (lookup v_upd e) ((v \<Midarrow> v') \<sqinter> (e \<mapsto> v'))"
+  by (auto simp: lookup_def valid_mem_def singleton_def intro!: sl)
+
+lemma sl_lookup_lkl [sl]: "vars1 v_upd v \<Longrightarrow> vars3 v_upd v'' \<Longrightarrow> free v_upd e \<Longrightarrow>
+    ht ((v \<Midarrow> v') \<sqinter> (e \<mapsto> v'')) (lookup v_upd e) ((v \<Midarrow> v'') \<sqinter> (subst e v_upd v' \<mapsto> v))"
+  by (auto simp: lookup_def valid_mem_def singleton_def intro!: sl)
+
+lemma sl_lookup [sl]: "ht (EXS v'. (e \<mapsto> v') * ((e \<mapsto> v') -* (subst_pred r v_upd v'))) (lookup v_upd e) r"
+  apply (auto simp: lookup_def intro!: sl)
+  apply (subgoal_tac "(a, b) \<in> subst_pred r v_upd x")
+  prefer 2
+  using bbi.sep_impl_annil1 apply blast
+  apply auto
+  apply (clarsimp simp: valid_mem_def)
+  prefer 2
+  apply (clarsimp simp: valid_mem_def)
+  apply (clarsimp simp: sep_def singleton_def)
+  apply (rule_tac x="x a" in exI)
+  apply (simp add: heap_divider)
+  apply (subgoal_tac "y = x a")
+  apply simp
+  apply (clarsimp simp: sep_def singleton_def)
+  apply auto
+  by (simp add: domI ortho_def)
+
+
+lemma sl_lookup_alt [sl]: "ht (EXS v'. (e \<hookrightarrow> v') \<sqinter> (subst_pred r v_upd v')) (lookup v_upd e) r"
+  apply (rule hl_pre)
+  prefer 2
+  apply (rule sl_lookup)
+  apply (rule Collect_mono)
+  apply (rule impI)
+  apply (erule exE)
+  apply (rule_tac x=xa in exI)
+  apply (rule impE)
+  prefer 2
+  apply assumption
+  prefer 2
+  apply assumption
+  apply (rule in_mono)
+  apply (rule reynolds5)
+done
+
+
+end
